Challenge/Ripemd160/Submission/Proofs/Bytecode/StackRoundData.lean
@@ -63,14 +63,14 @@ def leftHelperPCOfGroup (group : Nat) : UInt256 :=
   | 0 => UInt256.ofNat 0xfca
   | 1 => UInt256.ofNat 0xffe
   | 2 => UInt256.ofNat 0xe2d
-  | 3 => UInt256.ofNat 0x1052
-  | _ => UInt256.ofNat 0x108e
+  | 3 => UInt256.ofNat 0x1075
+  | _ => UInt256.ofNat 0x10b1
 
 def rightHelperPCOfGroup (group : Nat) : UInt256 :=
   match group with
   | 0 => UInt256.ofNat 0xedf
   | 1 => UInt256.ofNat 0x1127
-  | 2 => UInt256.ofNat 0xf3a
+  | 2 => UInt256.ofNat 0xf56
   | 3 => UInt256.ofNat 0xf91
   | _ => UInt256.ofNat 0xfcd
 
